feat: interpretation soundness

GroupoidModel/Russell_PER_MS/Interpretation.lean
@@ -1,4 +1,4 @@
-import GroupoidModel.Russell_PER_MS.Typing
+import GroupoidModel.Russell_PER_MS.Lemmas
 import GroupoidModel.Russell_PER_MS.UHom
 
 import GroupoidModel.ForMathlib
@@ -9,20 +9,23 @@ open CategoryTheory Limits
 
 noncomputable section
 
-namespace NaturalModelBase.UHomSeq
+namespace NaturalModelBase
+namespace UHomSeq
 
-variable {Ctx : Type u} [Category.{v, u} Ctx] [HasTerminal Ctx]
+variable {𝒞 : Type u} [Category.{v, u} 𝒞] [HasTerminal 𝒞]
+
+/-! ## Context stacks -/
 
 /-- `s.CtxStack Γ` witnesses a sequence of context extension operations in `s`
 that built the semantic context `Γ`. -/
-inductive CtxStack (s : UHomSeq Ctx) : Ctx → Type (max u v) where
-  | nil : CtxStack s (⊤_ Ctx)
+inductive CtxStack (s : UHomSeq 𝒞) : 𝒞 → Type (max u v) where
+  | nil : CtxStack s (⊤_ 𝒞)
   | cons {Γ} {l : Nat} (llen : l < s.length + 1) (A : y(Γ) ⟶ s[l].Ty) :
     CtxStack s Γ → CtxStack s (s[l].ext A)
 
-variable {s : UHomSeq Ctx}
+variable {s : UHomSeq 𝒞}
 
-protected def CtxStack.var {Γ : Ctx} {l : Nat} (llen : l < s.length + 1) :
+protected def CtxStack.var {Γ : 𝒞} {l : Nat} (llen : l < s.length + 1) :
     s.CtxStack Γ → ℕ → Part (y(Γ) ⟶ s[l].Tm)
   | .nil, _ => .none
   | .cons (l := l') _ A _, 0 =>
@@ -37,20 +40,35 @@ i.e., one of the form `1.Aₙ₋₁.….A₀`,
 together with the list `[Aₙ₋₁, …, A₀]`.
 
 This kind of context can be destructured. -/
-def CCtx (s : UHomSeq Ctx) : Type (max u v) := Σ Γ : Ctx, s.CtxStack Γ
+def CCtx (s : UHomSeq 𝒞) : Type (max u v) := Σ Γ : 𝒞, s.CtxStack Γ
 
-def CCtx.nil (s : UHomSeq Ctx) : s.CCtx :=
-  ⟨⊤_ Ctx, .nil⟩
+def nilCCtx (s : UHomSeq 𝒞) : s.CCtx :=
+  ⟨⊤_ 𝒞, .nil⟩
 
-def CCtx.cons (Γ : s.CCtx) {i : Nat} (ilen : i < s.length + 1)
-    (A : y(Γ.1) ⟶ s[i].Ty) : s.CCtx :=
-  ⟨s[i].ext A, .cons ilen A Γ.2⟩
+def CCtx.cons {l : Nat} (Γ : s.CCtx) (ilen : l < s.length + 1)
+    (A : y(Γ.1) ⟶ s[l].Ty) : s.CCtx :=
+  ⟨s[l].ext A, .cons ilen A Γ.2⟩
 
-protected def CCtx.var {l : Nat} (llen : l < s.length + 1) (Γ : s.CCtx) (i : ℕ) :
+protected def CCtx.var {l : Nat} (Γ : s.CCtx) (llen : l < s.length + 1) (i : ℕ) :
     Part (y(Γ.1) ⟶ s[l].Tm) :=
   Γ.2.var llen i
 
-variable [SmallCategory Ctx] [HasTerminal Ctx] (s : UHomSeqPis Ctx)
+variable (slen : univMax ≤ s.length)
+
+include slen in
+theorem lt_slen_of_eqTp {Γ A B l} : Γ ⊢[l] A ≡ B → l < s.length + 1 := by
+  intro Aeq
+  have := Aeq.le_univMax
+  omega
+
+end UHomSeq
+
+/-! ## Interpretation -/
+
+namespace UHomSeqPis
+
+variable {𝒞 : Type u} [SmallCategory 𝒞] [HasTerminal 𝒞]
+  {s : UHomSeqPis 𝒞}
 
 mutual
 
@@ -103,4 +121,269 @@ def ofTerm (Γ : s.CCtx) (l : Nat) :
 
 end
 
-end NaturalModelBase.UHomSeq
+def ofCtx (s : UHomSeqPis 𝒞) : Ctx → Part s.CCtx
+  | [] => return s.nilCCtx
+  | (A,l) :: Γ => do
+    Part.assert (l < s.length + 1) fun llen => do
+    let sΓ ← s.ofCtx Γ
+    let sA ← ofType sΓ l A
+    return sΓ.cons llen sA
+
+theorem cons_mem_ofCtx {Γ A l llen sΓ sA} : sΓ ∈ s.ofCtx Γ → sA ∈ ofType sΓ l A llen →
+    sΓ.cons llen sA ∈ s.ofCtx ((A,l) :: Γ) := by
+  simp only [ofCtx, Part.pure_eq_some, Part.bind_eq_bind, Part.mem_assert_iff, Part.mem_bind_iff,
+    Part.mem_some_iff]
+  tauto
+
+theorem mem_var_of_lookup {Γ A i l llen sΓ sA} : Lookup Γ i A l →
+    sΓ ∈ s.ofCtx Γ → sA ∈ ofType sΓ l A llen →
+    ∃ sv, sv ∈ (sΓ.var llen i) ∧ sv ≫ s[l].tp = sA := by
+  intro lk sΓmem sAmem
+  induction lk
+  . sorry
+  . sorry
+
+/-! ## Semantic substitution -/
+
+
+
+theorem mem_ofType_inst {A B t l l' llen l'len} {sΓ sA sB st}
+    (sA_mem : sA ∈ ofType sΓ l A llen)
+    (st_mem : st ∈ ofTerm sΓ l t llen) (st_tp : st ≫ s[l].tp = sA)
+    (sB_mem : sB ∈ ofType (sΓ.cons llen sA) l' B l'len) :
+    s[l].inst sA sB st st_tp ∈ ofType sΓ l' (B.inst t) l'len := by
+  sorry
+
+theorem mem_ofTerm_inst {A B t a l l' llen l'len} {sΓ sA sB st sa}
+    (sA_mem : sA ∈ ofType sΓ l A llen)
+    (st_mem : st ∈ ofTerm sΓ l t llen) (st_tp : st ≫ s[l].tp = sA)
+    (sB_mem : sB ∈ ofType (sΓ.cons llen sA) l' B l'len)
+    (sa_mem : sa ∈ ofTerm (sΓ.cons llen sA) l' a l'len) (sa_tp : sa ≫ s[l'].tp = sB) :
+    s[l].inst sA sa st st_tp ∈ ofTerm sΓ l' (a.inst t) l'len :=
+  sorry
+
+theorem mem_ofType_lift {A B l l' llen l'len} {sΓ sA sB}
+    (sA_mem : sA ∈ ofType sΓ l A llen)
+    (sB_mem : sB ∈ ofType sΓ l' B l'len) :
+    (s[l']'l'len).wk sB sA ∈ ofType (sΓ.cons l'len sB) l (A.lift) llen :=
+  sorry
+
+theorem mem_ofTerm_lift {A B t l l' llen l'len} {sΓ sA sB st}
+    (sA_mem : sA ∈ ofType sΓ l A llen)
+    (st_mem : st ∈ ofTerm sΓ l t llen)
+    (sB_mem : sB ∈ ofType sΓ l' B l'len) :
+    (s[l']'l'len).wk sB st ∈ ofTerm (sΓ.cons l'len sB) l (t.lift) llen :=
+  sorry
+
+/-! ## Soundness of interpretation -/
+
+variable (slen : univMax ≤ s.length)
+
+macro "simp_part" : tactic =>
+  `(tactic| simp only [Part.mem_assert_iff, Part.mem_bind_iff, Part.mem_some_iff,
+    exists_true_left, exists_const])
+macro "simp_part" loc:Lean.Parser.Tactic.location : tactic =>
+  `(tactic| simp only [Part.mem_assert_iff, Part.mem_bind_iff, Part.mem_some_iff,
+    exists_true_left, exists_const] $loc)
+
+theorem mem_ofTerm_app {B f a} {i j : Nat} (ilen : i < s.length + 1) (jlen : j < s.length + 1)
+    {sΓ : s.CCtx} {sA : y(sΓ.1) ⟶ s[i].Ty} {sB : y((sΓ.cons ilen sA).1) ⟶ (s[j]'jlen).Ty}
+    {sf : y(sΓ.1) ⟶ s[max i j].Tm} {sa : y(sΓ.1) ⟶ (s[i]'ilen).Tm}
+    (sB_mem : sB ∈ ofType (sΓ.cons ilen sA) j B jlen)
+    (sf_mem : sf ∈ ofTerm sΓ (max i j) f (by skip) /- wtf -/)
+    (sf_tp : sf ≫ s[max i j].tp = s.mkPi ilen jlen sA sB)
+    (sa_mem : sa ∈ ofTerm sΓ i a ilen)
+    (sa_tp : sa ≫ s[i].tp = sA) :
+    s.mkApp ilen jlen sA sB sf sf_tp sa sa_tp ∈ ofTerm sΓ j (.app i j B f a) jlen := by
+  cases sa_tp
+  dsimp [ofTerm]
+  simp_part
+  use ilen, sf, sf_mem, sa, sa_mem, sB, sB_mem, sf_tp
+
+theorem mem_ofTerm_lam {A t} {i j : Nat} (ilen : i < s.length + 1) (jlen : j < s.length + 1)
+    {sΓ : s.CCtx} {sA : y(sΓ.1) ⟶ (s[i]'ilen).Ty} {st : y((sΓ.cons ilen sA).1) ⟶ (s[j]'jlen).Tm}
+    (sA_mem : sA ∈ ofType sΓ i A ilen)
+    (st_mem : st ∈ ofTerm (sΓ.cons ilen sA) j t jlen) :
+    s.mkLam ilen jlen sA st ∈ ofTerm sΓ (max i j) (.lam i j A t) (by skip) := by
+  dsimp [ofTerm]
+  simp_part
+  use sA, sA_mem, st, st_mem
+
+-- TODO: this proof is boring, repetitive exists-elim/exists-intro: automate!
+theorem ofType_ofTerm_sound :
+    (∀ {Γ l A B}, (Aeq : Γ ⊢[l] A ≡ B) → ∀ {sΓ}, sΓ ∈ ofCtx s Γ →
+      have llen := s.lt_slen_of_eqTp slen Aeq
+      ∃ sA ∈ ofType sΓ l A llen, sA ∈ ofType sΓ l B llen) ∧
+    (∀ {Γ l t u A}, (teq : Γ ⊢[l] t ≡ u : A) → ∀ {sΓ}, sΓ ∈ ofCtx s Γ →
+      have llen := s.lt_slen_of_eqTp slen teq.wf_tp
+      ∃ sA ∈ ofType sΓ l A llen, ∃ st ∈ ofTerm sΓ l t llen,
+        st ∈ ofTerm sΓ l u llen ∧ st ≫ s[l].tp = sA) := by
+
+  have cons_helper {Γ A A' l sΓ} :
+      (Aeq : Γ ⊢[l] A ≡ A') → sΓ ∈ ofCtx s Γ →
+        have llen := s.lt_slen_of_eqTp slen Aeq
+        ∀ {sA}, sA ∈ ofType sΓ l A llen → sΓ.cons llen sA ∈ ofCtx s ((A, l) :: Γ) :=
+    fun Aeq sΓmem {sA} sAmem =>
+      have llen := s.lt_slen_of_eqTp slen Aeq
+      have sΓA := sΓ.cons llen sA
+      cons_mem_ofCtx sΓmem sAmem
+
+  refine
+    ⟨@EqTp.rec (fun Γ l A B _ => _) (fun Γ l t u A _ => _)
+      ?cong_pi ?cong_univ ?cong_el ?inst_tp ?symm_tp ?trans_tp ?cong_bvar ?cong_lam ?cong_app
+      ?cong_code ?app_lam ?eta ?conv ?inst_tm ?symm_tm ?trans_tm,
+    @EqTm.rec (fun Γ l A B _ => _) (fun Γ l t u A _ => _)
+      ?cong_pi ?cong_univ ?cong_el ?inst_tp ?symm_tp ?trans_tp ?cong_bvar ?cong_lam ?cong_app
+      ?cong_code ?app_lam ?eta ?conv ?inst_tm ?symm_tm ?trans_tm⟩
+
+  case eta =>
+    intros; intros
+    rename_i l l' twf ihf _ sΓmem _
+    have ⟨sAB, sABmem, sf, sfmem, sfmem', sftp⟩ := ihf sΓmem
+    have maxlen := s.lt_slen_of_eqTp slen twf.wf_tp
+    have llen : l < s.length + 1 := by omega
+    have l'len : l' < s.length + 1 := by omega
+    have sABmem_ := sABmem
+    dsimp [ofType] at sABmem
+    simp_part at sABmem
+    have ⟨sA, sAmem, sB, sBmem, sABeq⟩ := sABmem
+    refine ⟨sAB, sABmem_, sf, sfmem, ?_, sftp⟩
+    dsimp [ofTerm]
+    simp_part
+    use sA, sAmem
+    have vtp : s[l].var sA ≫ s[l].tp = s[l].wk sA sA := by simp
+    have wkAmem := mem_ofType_lift sAmem sAmem
+    use s.mkApp llen l'len (s[l].wk sA sA) (s[l].wk _ sB) (s[l].wk sA sf) sorry (s[l].var sA) vtp
+    refine ⟨⟨llen,
+        ⟨_, mem_ofTerm_lift sABmem_ sfmem sAmem,
+        s[l].var sA, ?_,
+        _, mem_ofType_lift sBmem (vtp ▸ wkAmem),
+        ?_,
+        ?_⟩⟩,
+      ?_⟩
+    . simp [UHomSeq.CCtx.var, UHomSeq.CtxStack.var]
+      rfl
+    . sorry -- same sorry as above
+    . convert rfl
+    . dsimp [mkApp]
+      sorry -- need another lemma
+
+  all_goals intros; dsimp [ofType]; try intros
+  case cong_pi Aeq Beq ihA ihB sΓ sΓmem =>
+    have ⟨sA, sAmem, sAmem'⟩ := ihA sΓmem
+    have ⟨sB, sBmem, sBmem'⟩ := ihB (cons_helper Aeq sΓmem sAmem)
+    have llen := s.lt_slen_of_eqTp slen Aeq
+    have l'len := s.lt_slen_of_eqTp slen Beq
+    use s.mkPi llen l'len sA sB
+    simp_part
+    constructor
+    . use sA, sAmem, sB, sBmem
+    . use sA, sAmem', sB, sBmem'
+  case cong_univ => simp
+  case cong_el Aeq ih _ sΓmem =>
+    have ⟨sU, sUmem, sA, sAmem, sAmem', sAtp⟩ := ih sΓmem
+    have llen := Nat.succ_lt_succ_iff.mp <| s.lt_slen_of_eqTp slen Aeq.wf_tp
+    dsimp [ofType] at sUmem
+    simp_part at sUmem
+    use s.el llen sA (sUmem ▸ sAtp)
+    simp_part
+    simp only [llen, exists_true_left]
+    exact ⟨⟨sA, sAmem, sAtp.trans sUmem, rfl⟩, sA, sAmem', sAtp.trans sUmem, rfl⟩
+  case inst_tp teq ihB iht sΓ sΓmem =>
+    have ⟨sA, sAmem, st, stmem, stmem', sttp⟩ := iht sΓmem
+    have ⟨sB, sBmem, sBmem'⟩ := ihB (cons_helper teq.wf_tp sΓmem sAmem)
+    exact ⟨_, mem_ofType_inst sAmem stmem sttp sBmem, mem_ofType_inst sAmem stmem' sttp sBmem⟩
+  case symm_tp ih _ sΓmem =>
+    have ⟨sA, sAmem, sAmem'⟩ := ih sΓmem
+    exact ⟨sA, sAmem', sAmem⟩ -- `use` fails here?
+  case trans_tp ih ih' _ sΓmem =>
+    have ⟨sA, sAmem, sAmem'⟩ := ih sΓmem
+    have ⟨sA', sA'mem, sA'mem'⟩ := ih' sΓmem
+    use sA, sAmem
+    convert sA'mem'
+    exact Part.mem_unique sAmem' sA'mem
+  case cong_bvar lk ihA _ sΓmem =>
+    have ⟨sA, sAmem, sAmem'⟩ := ihA sΓmem
+    have ⟨sv, svmem, svtp⟩ := mem_var_of_lookup lk sΓmem sAmem
+    use sA, sAmem, sv, svmem, svmem, svtp
+  case cong_lam Aeq teq ihA iht sΓ sΓmem =>
+    have ⟨sA, sAmem, sAmem'⟩ := ihA sΓmem
+    have ⟨sB, sBmem, st, stmem, stmem', sttp⟩ := iht (cons_helper Aeq sΓmem sAmem)
+    have llen := s.lt_slen_of_eqTp slen Aeq
+    have l'len := s.lt_slen_of_eqTp slen teq.wf_tp
+    simp_part
+    use s.mkPi llen l'len sA sB
+    refine ⟨⟨sA, sAmem, sB, sBmem, rfl⟩,
+      _, mem_ofTerm_lam llen l'len sAmem stmem,
+      mem_ofTerm_lam llen l'len sAmem' stmem',
+      ?_⟩
+    simp [sttp]
+  case cong_app Beq _ aeq ihB ihf iha _ sΓmem =>
+    dsimp [ofTerm]
+    have ⟨sA, sAmem, sa, samem, samem', satp⟩ := iha sΓmem
+    have ⟨sB, sBmem, sBmem'⟩ := ihB (cons_helper aeq.wf_tp sΓmem sAmem)
+    have ⟨sAB, sABmem, sf, sfmem, sfmem', sftp⟩ := ihf sΓmem
+    dsimp [ofType] at sABmem
+    simp_part at sABmem
+    have ⟨sA', sA'mem, sB', sB'mem, sABeq⟩ := sABmem
+    cases Part.mem_unique sA'mem sAmem
+    cases Part.mem_unique sB'mem sBmem
+    cases sABeq
+    cases satp
+    have llen := s.lt_slen_of_eqTp slen aeq.wf_tp
+    have l'len := s.lt_slen_of_eqTp slen Beq
+    simp_part
+    refine ⟨_, mem_ofType_inst sAmem samem rfl sBmem,
+      s.mkApp llen l'len _ sB sf sftp sa rfl,
+      ⟨llen, sf, sfmem, sa, samem, sB, sBmem, sftp, rfl⟩,
+      ⟨llen, sf, sfmem', sa, samem', sB, sBmem', sftp, rfl⟩,
+      ?_⟩
+    simp
+  case cong_code lMax Aeq ih _ sΓmem =>
+    have ⟨sA, sAmem, sAmem'⟩ := ih sΓmem
+    dsimp [ofTerm]
+    simp_part
+    have llen := lMax.trans_le slen
+    refine ⟨_, rfl, s.code llen sA,
+      ⟨Nat.succ_pos _, sA, sAmem, rfl⟩,
+      ⟨Nat.succ_pos _, sA, sAmem', rfl⟩,
+      ?_⟩
+    erw [s.toUHomSeq.code_tp]
+  case app_lam twf uwf iht ihu _ sΓmem =>
+    have ⟨sA, sAmem, su, sumem, _, sutp⟩ := ihu sΓmem
+    have ⟨sB, sBmem, st, stmem, _, sttp⟩ := iht (cons_helper uwf.wf_tp sΓmem sAmem)
+    have llen := s.lt_slen_of_eqTp slen uwf.wf_tp
+    have l'len := s.lt_slen_of_eqTp slen twf.wf_tp
+    refine ⟨_, mem_ofType_inst sAmem sumem sutp sBmem,
+      _, mem_ofTerm_app llen l'len sBmem (mem_ofTerm_lam llen l'len sAmem stmem) ?_ sumem sutp,
+      ?_, ?_⟩
+    . simp [sttp]
+    . rw [mkApp_mkLam (t_tp := sttp)]
+      exact mem_ofTerm_inst sAmem sumem sutp sBmem stmem sttp
+    . simp
+  case conv ihA iht sΓ sΓmem =>
+    have ⟨sA, sAmem, sAmem'⟩ := ihA sΓmem
+    have ⟨sA_, sAmem_, st, stmem, stmem', sttp⟩ := iht sΓmem
+    use sA, sAmem', st, stmem, stmem'
+    convert sttp
+    exact Part.mem_unique sAmem sAmem_
+  case inst_tm l _ _ teq iha iht sΓ sΓmem =>
+    have ⟨sA, sAmem, st, stmem, stmem', sttp⟩ := iht sΓmem
+    have ⟨sB, sBmem, sa, samem, samem', satp⟩ := iha (cons_helper teq.wf_tp sΓmem sAmem)
+    have llen := s.lt_slen_of_eqTp slen teq.wf_tp
+    refine ⟨_, mem_ofType_inst sAmem stmem sttp sBmem, _,
+      mem_ofTerm_inst sAmem stmem sttp sBmem samem satp,
+      mem_ofTerm_inst sAmem stmem' sttp sBmem samem' satp,
+      s[l].inst_tp sA sB sa satp st sttp⟩
+  case symm_tm ih _ sΓmem =>
+    have ⟨sA, sAmem, st, stmem, stmem', sttp⟩ := ih sΓmem
+    use sA, sAmem, st, stmem', stmem, sttp
+  case trans_tm ih ih' _ sΓmem =>
+    have ⟨sA, sAmem, st, stmem, stmem', sttp⟩ := ih sΓmem
+    have ⟨sA', sA'mem, st', st'mem, st'mem', st'tp⟩ := ih' sΓmem
+    refine ⟨sA, sAmem, st, stmem, ?_, sttp⟩
+    convert st'mem'
+    exact Part.mem_unique stmem' st'mem
+
+end UHomSeqPis
+end NaturalModelBase
