GroupoidModel/Russell_PER_MS/Lemmas.lean
@@ -11,16 +11,16 @@ theorem EqTm.le_univMax {Γ A t u l} : Γ ⊢[l] t ≡ u : A → l ≤ univMax :
   all_goals intros; first| trivial | omega
 
 theorem EqTp.wf_left {Γ A B l} : Γ ⊢[l] A ≡ B → Γ ⊢[l] A :=
-  fun h => .trans h (.symm h)
+  fun h => .trans_tp h (.symm_tp h)
 
 theorem EqTp.wf_right {Γ A B l} : Γ ⊢[l] A ≡ B → Γ ⊢[l] B :=
-  fun h => .trans (.symm h) h
+  fun h => .trans_tp (.symm_tp h) h
 
 theorem EqTm.wf_left {Γ A t u l} : Γ ⊢[l] t ≡ u : A → Γ ⊢[l] t : A :=
-  fun h => .trans h (.symm h)
+  fun h => .trans_tm h (.symm_tm h)
 
 theorem EqTm.wf_right {Γ A t u l} : Γ ⊢[l] t ≡ u : A → Γ ⊢[l] u : A :=
-  fun h => .trans (.symm h) h
+  fun h => .trans_tm (.symm_tm h) h
 
 theorem EqTm.wf_tp {Γ A t u l} : Γ ⊢[l] t ≡ u : A → Γ ⊢[l] A := by
   apply @EqTm.rec
@@ -30,12 +30,12 @@ theorem EqTm.wf_tp {Γ A t u l} : Γ ⊢[l] t ≡ u : A → Γ ⊢[l] A := by
   case cong_lam A_eq _ _ B_wf =>
     exact .cong_pi A_eq.wf_left B_wf
   case cong_app B_eq _ a_eq _ _ _ =>
-    exact (EqTp.inst B_eq a_eq).wf_left
+    exact (EqTp.inst_tp B_eq a_eq).wf_left
   case cong_code =>
     apply EqTp.cong_univ; assumption
-  case inst a_eq B_wf _ =>
-    exact (EqTp.inst B_wf a_eq).wf_left
+  case inst_tm a_eq B_wf _ =>
+    exact (EqTp.inst_tp B_wf a_eq).wf_left
   case app_lam u_wf B_wf _ =>
-    exact EqTp.inst B_wf u_wf
+    exact EqTp.inst_tp B_wf u_wf
   case conv A_eq _ _ _ =>
     exact A_eq.wf_right
